teaching/mpri-2-30/FStar/Calc.fst
@@ -1,0 +1,43 @@
+module Calc
+
+open FStar.Mul
+
+#reset-options "--z3rlimit 50"
+
+let rec pow2 (x: nat) : Tot pos =
+  match x with
+  | 0 -> 1
+  | _ -> 2 * (pow2 (x - 1))
+
+// BEGIN: Basic math lemmas
+assume val distributivity_add_left: a:int -> b:int -> c:int -> Lemma ((a + b) * c = a * c + b * c)
+
+assume val distributivity_add_right: a:int -> b:int -> c:int -> Lemma (a * (b + c) = a * b + a * c)
+
+assume val paren_mul_right: a:int -> b:int -> c:int -> Lemma (a * b * c = a * (b * c))
+
+assume val pow2_plus: n:nat -> m:nat -> Lemma (pow2 n * pow2 m = pow2 (n + m))
+
+assume val swap_mul: a:int -> b:int -> Lemma (a * b = b * a)
+
+assume val euclidean_division_definition: a:int -> b:nonzero -> Lemma (a = (a / b) * b + a % b)
+// END: Basic math lemmas
+
+
+val lemma_distr_pow (a b:int) (c d:nat) : Lemma ((a + b * pow2 c) * pow2 d = a * pow2 d + b * pow2 (c + d))
+let lemma_distr_pow a b c d = admit()
+
+val lemma_distr_pow_pow (a:int) (b:nat) (c:int) (d e:nat) :
+  Lemma ((a * pow2 b + c * pow2 d) * pow2 e = a * pow2 (b + e) + c * pow2 (d + e))
+let lemma_distr_pow_pow a b c d e = admit()
+
+val lemma_as_nat64_horner (r0 r1 r2 r3:int) :
+  Lemma (r0 + r1 * pow2 64 + r2 * pow2 128 + r3 * pow2 192 ==
+    ((r3 * pow2 64 + r2) * pow2 64 + r1) * pow2 64 + r0)
+let lemma_as_nat64_horner r0 r1 r2 r3 = admit()
+
+val lemma_distr_eucl_mul (r a:int) (b:pos) : Lemma (r * (a % b) + r * (a / b) * b = r * a)
+let lemma_distr_eucl_mul r a b = admit()
+
+val lemma_distr_eucl_mul_add (r a c:int) (b:pos) : Lemma (r * (a % b) + r * (a / b + c) * b = r * a + r * c * b)
+let lemma_distr_eucl_mul_add r a c b = admit()
