teaching/mpri-2-30/FStar/Stack.fsti
@@ -1,0 +1,15 @@
+module Stack
+
+// BEGIN: stack_types
+val stack : Type0  (* type of stacks *)
+
+val empty : stack
+val is_empty : stack -> GTot bool
+
+val push : int -> stack -> stack
+val pop : stack -> option stack
+val top : stack -> option int
+// END: stack_types
+
+// BEGIN: stack_lemmas
+// END: stack_lemmas
